loop init

theories/examples/copy_word.v
@@ -145,43 +145,246 @@ Section copy_word.
      - loop rule ???
      - branch rule ???
    *)
-  (*
-  Definition cmp_I ra := encode_instruction (Cmp ra).
+  
+  Definition cmp_I ra v := encode_instruction (Cmp ra (inr v)).
   Definition bne_I ra := encode_instruction (Bne ra).
-  Definition sub_word_I ra w := encode_instruction (Sub ra (inl w)).
-  Definition add_word_I ra w := encode_instruction (Add ra (inl w)).
-  Definition sub_reg_I ra rb := encode_instruction (Sub ra (inr rb)).
-  Definition add_reg_I ra rb := encode_instruction (Add ra (inr rb)).
+  Definition sub_reg_I ra rb := encode_instruction (Sub ra rb).
+  Definition add_reg_I ra rb := encode_instruction (Add ra rb).
   Definition mov_reg_I ra rb := encode_instruction (Mov ra (inr rb)).
+
+  Program Definition I0 : Imm := (I (finz.FinZ 0 _ _) _).
+  Solve Obligations with (try lia; solve_finz).
+
+  Program Definition I1 : Imm := (I (finz.FinZ 1 _ _) _).
+  Solve Obligations with (try lia; solve_finz).
+
+  Program Definition I2 : Imm := (I (finz.FinZ 2 _ _) _).
+  Solve Obligations with (try lia; solve_finz).
+
+  Definition c_pre step :=
+    [
+    mov_word_I R5 step; (* remaining runs *)
+    mov_word_I R6 I0;    (* counter *)
+(*    mov_word_I R7 base    (* program base address *) *)
+    ].
+
+  Definition c_post :=
+    [
+    (* incr counter *)
+    mov_word_I R8 I1;
+    add_reg_I R6 R8;
+    (* conditional jump *)
+    (* might be a good idea to have a separate rule for branches *)
+    cmp_I R6 R5;
+    bne_I R7
+    ].
+
+  Definition cycle prog step := c_pre step ++ prog ++ c_post.
+
+  Lemma c_loop {progpage sacc i q} {n : nat} (body : list Word) step prog (P : Word -> iProp Σ) :
+    n = Z.to_nat (finz.to_z (of_imm step)) ->
+    (1 <= step)%Z ->
+    progpage ∈ sacc ->
+    seq_in_page (of_pid progpage) (length (cycle prog step)) progpage ->
+    (∀ v, ⌜(v <= step)%f⌝ -∗ {PAR{{ (P v) ∗ PC @@ i ->r ((of_pid progpage) ^+ 3)%f
+                         ∗ R6 @@ i ->r v
+                         ∗ R5 @@ i ->r step
+                         ∗ R7 @@ i ->r ((of_pid progpage) ^+ 2)%f
+                         ∗ R8 @@ i ->r I2                     
+                         ∗ A@i :={q}[sacc]
+                         ∗ (program' (cycle prog step) (of_pid progpage))
+            }}} ExecI @ i
+    {{{ RET ExecI; (P (v ^+ 1)%f) ∗ PC @@ i ->r (((of_pid progpage) ^+ 2)%f ^+ (length prog))%f
+                         ∗ R6 @@ i ->r v
+                         ∗ R5 @@ i ->r step
+                         ∗ R7 @@ i ->r ((of_pid progpage) ^+ 2)%f
+                         ∗ (∃ r, R8 @@ i ->r r)
+                         ∗ A@i :={q}[sacc]
+                         ∗ (program' (cycle prog step) (of_pid progpage))
+    }}}%I)
+    ⊢  {PAR{{ (P I0) ∗ PC @@ i ->r (of_pid progpage)
+                       ∗ (∃ r5, R5 @@ i ->r r5)
+                       ∗ (∃ r6, R6 @@ i ->r r6)
+                       ∗ (∃ r7, R7 @@ i ->r r7)
+                       ∗ (∃ r8, R8 @@ i ->r r8)
+                       ∗ A@i :={q}[sacc]
+                       ∗ program' (cycle prog step) (of_pid progpage)
+       }}} ExecI @ i
+    {{{ RET ExecI; (P step) ∗ PC @@ i ->r (of_pid progpage ^+ (length (cycle prog step)))%f
+                          ∗ R5 @@ i ->r step
+                          ∗ R6 @@ i ->r step
+                          ∗ R7 @@ i ->r ((of_pid progpage) ^+ 2)%f
+                          ∗ R8 @@ i ->r I2               
+                          ∗ A@i :={q}[sacc]
+                          ∗ program' (cycle prog step ((of_pid progpage) ^+ 2)%f) (of_pid progpage)
+    }}}%I.
+  Proof.
+    iIntros (Hn Hle Hprpain Hseq) "#Htriple".
+    generalize dependent step.
+    induction n.
+    - intros step eq c.
+      lia.
+    - intros step eq c seq.
+      iIntros (Φ).
+      iModIntro.
+      iIntros "(HPstep & Hpc & [% Hr5] & [% Hr6] & [% Hr7] & [% Hr8] & Hacc & Hprog)".
+      assert (Hn : n = Z.to_nat (step ^- 1)%f).
+      {
+        rewrite /decr_default.
+        rewrite /decr.
+        destruct (Z_le_dec 0%Z (step - 1)%Z) eqn:heq; [|lia].
+        destruct (Z_lt_dec (step - 1)%Z 2000000%Z).
+        - simpl.
+          lia.
+        - exfalso.
+          apply n0.
+          destruct step.
+          simpl.
+          destruct (decide ((w < 1000000)%Z)); [|lia].
+          lia.
+      } 
+      iIntros "Hϕ".
+    apply seq_in_page_forall in seq.
+    rewrite <-parwp_sswp.
+    iDestruct "Hprog" as "(p_start & Hprog)".
+    iDestruct ((mov_word (of_pid progpage) step R5) with "[Hpc Hacc Hr5 p_start]") as "J".
+    3 : { rewrite ->Forall_forall in seq. apply seq. set_solver. }
+    3 : { apply Hprpain. }
+    3 : { iFrame. }
+    auto.
+    by rewrite decode_encode_instruction.
+    iApply "J".
+    iModIntro.
+    iIntros "(Hpc & Hinstr1 & Hacc & Hr5)".
+    rewrite <-parwp_sswp.
+    iDestruct "Hprog" as "(p_start & Hprog)".
+    iDestruct ((mov_word ((of_pid progpage ^+ 1)%f) I0 R6) with "[Hpc Hacc Hr6 p_start]") as "J".
+    3 : { rewrite ->Forall_forall in seq. apply seq. set_solver. }
+    3 : { apply Hprpain. }
+    3 : { iFrame. }
+    auto.
+    by rewrite decode_encode_instruction.
+    iApply "J".
+    iModIntro.
+    iIntros "(Hpc & Hinstr2 & Hacc & Hr6)".
+    rewrite <-parwp_sswp.
+    iDestruct "Hprog" as "(p_start & Hprog)".
+    iDestruct ((mov_reg (((of_pid progpage ^+ 1) ^+ 1)%f) ((of_pid progpage ^+ 1) ^+ 1)%f PC R7) with "[Hpc Hacc Hr7 p_start]") as "J".
+    3 : { rewrite ->Forall_forall in seq. apply seq. set_solver. }
+    3 : { apply Hprpain. }
+    3 : { iFrame. }
+    auto.
+    by rewrite decode_encode_instruction.
+    iApply "J".
+    iModIntro.
+    iDestruct ((ldr (of_pid progpage ^+ 1)%f src R1 R0) with "[Hpc Hacc Hr0 Hr1 Hsrc p_start HTX]") as "J".
+    instantiate (1 := Ldr R1 R0).
+    reflexivity.
+    instantiate (1 := encode_instruction (Ldr R1 R0)).
+    by rewrite decode_encode_instruction.
+    instantiate (1 := ptx).
+    intros C.
+    apply to_pid_aligned_in_page in Hsrcp.
+    rewrite <-Hsrcp in Hneq.
+    rewrite C in Hneq.
+    apply Hneq.
+    reflexivity.
+    rewrite ->Forall_forall in Hseqp.
+    specialize (Hseqp (progpage ^+ 1)%f).
+    instantiate (1 := sacc).
+    apply to_pid_aligned_in_page in Hsrcp.
+    subst srcpage.
+    assert (Hp : (progpage ^+ 1)%f ∈ finz.seq progpage (length (program src dst))).
+    set_solver.
+    specialize (Hseqp Hp).
+    apply to_pid_aligned_in_page in Hseqp.
+    rewrite Hseqp.
+    set_solver.
+    iFrame.
+    iApply "J".
+    iModIntro.
+    iIntros "(Hpc & Hinstr2 & Hr0 & Hsrc & Hr1 & Hacc & HTX)".
+    rewrite <-parwp_sswp.
+    iDestruct "Hbstar" as "(p_start & Hbstar)".
+    iDestruct ((mov_word ((of_pid progpage ^+ 1) ^+ 1)%f dst R0) with "[Hpc Hacc Hr0 p_start]") as "J".
+    3 : { rewrite ->Forall_forall in Hseqp. apply Hseqp. set_solver. }
+    3 : { apply Hprpain. }
+    3 : { iFrame. }
+    auto.
+    by rewrite decode_encode_instruction.
+    iApply "J".
+    iModIntro.
+    iIntros "(Hpc & Hinstr3 & Hacc & Hr0)".
+    rewrite <-parwp_sswp.
+    iDestruct "Hbstar" as "(p_start & Hbstar)".
+    iDestruct ((str (((of_pid progpage ^+ 1) ^+ 1) ^+ 1)%f dst R1 R0) with "[Hpc Hacc Hr0 p_start Hdst Hr1 HRX]") as "J".
+    instantiate (1 := Str R1 R0).
+    reflexivity.
+    instantiate (1 := encode_instruction (Str R1 R0)).
+    by rewrite decode_encode_instruction.
+    instantiate (1 := prx).
+    intros C.
+    rewrite C in Hneq'.
+    apply Hneq'.
+    apply to_pid_aligned_in_page in Hdstp.
+    assumption.
+    instantiate (1 := sacc).
+    apply to_pid_aligned_in_page in Hdstp.
+    subst dstpage.
+    rewrite ->Forall_forall in Hseqp.
+    specialize (Hseqp (((progpage ^+ 1) ^+ 1) ^+ 1)%f).
+    pose proof (to_pid_aligned_in_page (((progpage ^+ 1) ^+ 1) ^+ 1)%f progpage) as Hp.
+    assert (Hq : (((progpage ^+ 1) ^+ 1) ^+ 1)%f ∈ finz.seq progpage (length (program src dst))).
+    set_solver.
+    specialize (Hseqp Hq).
+    specialize (Hp Hseqp).
+    rewrite Hp.
+    set_solver.
+    iFrame.
+    iApply "J".
+    iModIntro.
+    iIntros "(Hpc & Hinstr4 & Hr0 & Hdst & Hr1 & Hacc & HRX)".
+    iApply parwp_finish.
+    iFrame.
+    iSplit; auto.
+    assert (Hp : (progpage ^+ length (program src dst))%f = ((((progpage ^+ 1) ^+ 1) ^+ 1) ^+ 1)%f).
+    assert (Hq : Z.of_nat (length (program src dst)) = 4%Z). by compute.
+    rewrite Hq.
+    solve_finz.
+    rewrite Hp.
+    iFrame.
+  Qed.
   
   Definition program_c step src dst :=
     [
-    mov_word_I R2 step; (* remaining runs *)
-    mov_word_I R4 0;    (* counter *)
-    mov_reg_I R3 PC;    (* program base address *)
-    add_I R3 2;         (* loop base address *)
+    mov_word_I R5 step; (* remaining runs *)
+    mov_word_I R6 I0;    (* counter *)
+    mov_reg_I R7 PC;    (* program base address *)
+    mov_word_I R8 I2;
+    add_reg_I R7 R8;         (* loop base address *)    
     (* loop body begin *)
     (* loop may depend on step and counter
-       it should restore PC, R2, R4
+       it should restore PC, R5, R6
        perhaps, we could try to write a special rule for loops
      *)
     (* ldr data from src + counter to R1 *)
-    mov_word_I R0 src;
-    add_I R0 R4;
-    ldr_I R1 R0;
+    mov_word_I R8 src;
+    add_reg_I R8 R6;
+    ldr_I R9 R8;
     (* str data from R1 to dst + counter *)
-    mov_word_I R0 dst;
-    add_I R0 R4;
-    str_I R1 R0;
-    (* loop body end *)
+    mov_word_I R8 dst;
+    add_reg_I R8 R6;
+    str_I R9 R8;
+    (* loop body end *)    
     (* incr counter *)
-    add_I R4 1;
+    mov_word_I R8 I1;
+    add_reg_I R6 R8;
     (* decr remaining runs *)
-    sub_I R2 1;
+    sub_reg_I R5 R8;
     (* conditional jump *)
     (* might be a good idea to have a separate rule for branches *)
-    cmp_I R2;
-    bne_I R3
+    cmp_I R5 I0;
+    bne_I R7
     ].
   
   Lemma copy_words {ptx prx progpage srcpage dstpage sacc i q qi w w_ r0_ r1_} step src dst :
